---
layout: post
title: 1974 USAMO 1
---
Let $$a$$, $$b$$, $$c$$ be three distinct integers, and let $$P$$ be a polynomial with integer
coefficients. Show that in this case the conditions $$P(a) = b$$, $$P(b) = c$$, $$P(c) = a$$ cannot be satisfied simultaneously.

Proof: we will use the fact that $$x-y$$|$$P(x)-P(y)$$

We have:

<<<<<<< HEAD
$$ a-b|P(a)-P(b) = b-c $$
$$ b-c|P(b)-P(c) = c-a $$
$$ c-a|P(c)-P(a) = a-b $$
=======
$$
a-b|P(a)-P(b) = b-c
b-c|P(b)-P(c) = c-a
c-a|P(c)-P(a) = a-b
$$
>>>>>>> 7e22ae482aeb4df3d27155fb2071b3f0d2e416f6

Thus, $$a-b|b-c|c-a|a-b \rightarrow a-b|b-c|a-b$$, so by symmetry
$$ b-c  = \pm(a-b) $$
$$ c-a =\pm(b-c) $$
$$ a-b = \pm(c-a) $$

If we had $$b-c=-(a-b)=b-a$$, we would have $$c=a$$, a contradiction, as $$a,b,c$$ are distinct.

Therefore,
$$ b-c = a-b $$
$$ c-a = b-c $$
$$ a-b = c-a $$
Thus,

$$ 2b = a+c $$
$$ 2c = b+a $$
$$ 2a = c+b $$

This is impossible, as plugging in $$2b-a=c$$ in the second equation yields:

$$ 2(2b-a)= b+a $$
$$ 4b-2a = b+a $$
$$ 3b = 3a $$
$$ b = a  $$

Which is a contradiction. Therefore,  $$P(a) = b$$, $$P(b) = c$$, $$P(c) = a$$ cannot be satisfied simultaneously. $$\square$$
